src/Parsers/DependentlyTypedOption.v
@@ -1,0 +1,60 @@
+(** * Transform CFG parser into an optional one *)
+Require Import Coq.Lists.List Coq.Program.Program Coq.Classes.RelationClasses Coq.Strings.String.
+Require Import Parsers.ContextFreeGrammar Parsers.Specification.
+Require Import Parsers.DependentlyTyped.
+Require Import Common.
+
+Set Implicit Arguments.
+
+Local Open Scope string_like_scope.
+
+Local Coercion is_true : bool >-> Sortclass.
+
+Section recursive_descent_parser.
+  Context {CharType : Type}
+          {String : string_like CharType}
+          {G : grammar CharType}.
+
+  Context {predata : parser_computational_predataT}.
+  Context {methods' : @parser_computational_dataT' _ String predata}.
+
+  (** some helper lemmas to help Coq with inference *)
+  Definition split_string_for_production_correct'
+             H0 H1 str0 valid it its str st
+    := @split_string_for_production_correct CharType String H0 H1 str0 valid it its {| string_val := str ; state_val := st |}.
+
+  Hint Unfold compose : dtp_option_db.
+  Hint Extern 1 => apply split_string_for_production_correct' : dtp_option_db.
+
+  Local Ltac t_option' :=
+    idtac;
+    match goal with
+      | _ => progress simpl
+      | _ => progress intros
+      | _ => progress destruct_head' @StringWithSplitState
+      | _ => progress destruct_head' option
+      | [ |- Forall _ (map _ _) ] => apply Forall_map
+      | _ => progress autounfold with dtp_option_db in *
+      | _ => solve [ eauto with dtp_option_db ]
+    end.
+
+  Local Ltac t_option := repeat t_option'.
+
+  Local Instance option_methods' : @parser_computational_dataT' _ String predata
+    := { split_stateT str0 valid g str := option (split_stateT str0 valid g str);
+         split_string_for_production str0 valid it its str
+         := match state_val str with
+              | None
+                => nil
+              | Some st
+                => map
+                     (fun s1s2 =>
+                        (lift_StringWithSplitState (fst s1s2) (@Some _),
+                         lift_StringWithSplitState (snd s1s2) (@Some _)))
+                     (split_string_for_production str0 valid it its {| string_val := string_val str ; state_val := st |})
+            end }.
+  Proof. clear; abstract t_option. Defined.
+
+  Local Instance option_methods : @parser_computational_dataT _ String
+    := { methods' := option_methods' }.
+End recursive_descent_parser.
